let-polymorphism.v
@@ -1,0 +1,53 @@
+Section Syntax.
+
+  Variable tvar : Type.
+
+  Inductive ty : Type :=
+  | TyVar : tvar -> ty
+  | TyLift : Type -> ty
+  | TyFun : ty -> ty -> ty.
+
+  Inductive tys : Type :=
+  | TysBase : ty -> tys
+  | TysForall : (tvar -> tys) -> tys.
+
+  Variable var : tys -> Type.
+
+  Inductive inst : tys -> ty -> Prop :=
+  | InstBase : forall (t : ty), inst (TysBase t) t
+  | InstForall : forall (f : tvar -> tys) (t : ty) (a : tvar), inst (f a) t -> inst (TysForall f) t.
+
+  Inductive expr : ty -> Type :=
+  | EVar : forall (s : tys) (t : ty), var s -> inst s t -> expr t
+  | EConst : forall (A : Type), A -> expr (TyLift A)
+  | EFun : forall (dom ran : ty), (var (TysBase dom) -> expr ran) -> expr (TyFun dom ran)
+  | EApp : forall (dom ran : ty), expr (TyFun dom ran) -> expr dom -> expr ran
+  | ELet : forall (s : tys) (t : ty), (forall (t' : ty), inst s t' -> expr t') -> (var s -> expr t) -> expr t.
+End Syntax.
+
+Check expr.
+
+Axiom todo : forall (A : Type), A.
+Definition tvar_basic := ty Type -> tys (ty Type).
+
+Lemma inst_EVvar :
+  inst tvar_basic
+    (TysForall tvar_basic
+       (fun a : tvar_basic =>
+          TysBase tvar_basic
+            (TyFun tvar_basic (TyVar tvar_basic a)
+               (TyVar tvar_basic a))))
+    (TyFun tvar_basic (TyLift tvar_basic nat)
+       (TyLift tvar_basic nat)).
+Proof.
+  econstructor.
+  try econstructor. (* cannot equate TyVar with TyLift *)
+Abort.
+
+Check (fun var =>
+         ELet tvar_basic var
+           (TysForall _ (fun a => TysBase _ (TyFun _ (TyVar _ a) (TyVar _ a))))
+           (TyLift _ nat)
+           (fun t' H_inst => todo _)
+           (fun f => EApp _ _ _ _ (EVar _ _ _ _ f (todo _)) (EConst _ _ _ 1))
+      ).
